Merge exceptions

coq-osiris/examples/proofs/exceptions.v
@@ -1,3 +1,6 @@
+(** This file contains both a "pure" and "effectful" proof of exceptions.v, to guide the
+   generalization of lemmas about [pure] to non-trivial exceptional postconditions.  *)
+
 From iris.proofmode Require Import base proofmode classes ltac_tactics.
 From iris.bi Require Import weakestpre.
 From iris Require Import base_logic.lib.gen_heap.
@@ -6,115 +9,209 @@ From osiris Require Import osiris.
 From osiris.stdlib Require Import Stdlib.
 From osiris.examples Require Import og_exception.
 
-(* TODO: We manually add exceptions to the environment. *)
-
 Definition stdlib_with_notfound :=
   ("Not_found", (VLoc (Loc 0))) :: stdlib_env.
 
-Section proof.
+Section proof_pure.
 
-Context `{!osirisGS Σ}.
+  (* Calling [head #l] either returns [#h] when [l = h :: t],
+    or throws an exception when [l = []]. *)
 
-(* Calling [head #l] either returns [#h] when [l = h :: t],
-   or throws an exception when [l = []]. *)
+  Definition head_spec head :=
+    ∀ (A : Type) (H : Encode A) (l : list A),
+      pure
+        (call head #l)
+        (λ h : A, exists t, l = h :: t)
+        (λ e, e = VXData (Loc 0) [] ∧ l = []).
 
-Definition head_spec head :=
-  ∀ (A : Type) (H : Encode A) (l : list A),
-    ⊢ ewp_def top (call head #l) ⊥
-      (| RET x => ∃ h t, ⌜l = h :: t /\ x = #h⌝ ;
-       | EXN e => ⌜e = VXData (Loc 0) [] /\ l = []⌝ )%I.
+  (* Calling [catch_head #l] either returns [Some #h] when [l = h ::t],
+    or returns [None] when [l = []]. *)
 
-(* Calling [catch_head #l] either returns [Some #h] when [l = h ::t],
-   or returns [None] when [l = []]. *)
+  Definition catch_head_spec catch_head :=
+    ∀ (A : Type) (H : Encode A) (l : list A),
+      pure
+        (call catch_head #l)
+        (λ hopt, hopt = list.head l) ⊥.
 
-Definition catch_head_spec catch_head :=
-  ∀ (A : Type) (H : Encode A) (l : list A),
-    ⊢ ewp_def top (call catch_head #l) ⊥
-      (RET #hopt, ⌜match l with
-                  | [] => hopt = None
-                  | h :: _ => hopt = Some h
-                  end⌝)%I.
+  (* TODO: MOVE? *)
+  Ltac set_pure_postcondition φ :=
+    match goal with
+      |- @pure ?A ?E ?m ?_φ ?ψ =>
+        let H := fresh in
+        cut (@pure A E m φ ψ); [ intro H; exact H | ]
+    end.
 
-Lemma example :
-  eval_module stdlib_with_notfound __main (λ η, True).
-Proof.
-  unfold __main.
-  apply module_struct.
+  Lemma example :
+    eval_module stdlib_with_notfound __main (λ η, True).
+  Proof.
+    unfold __main.
+    apply module_struct.
 
-  (* Struct item: [let head l = ...] *)
-  eapply structs_cons.
-  { apply struct_let_single with (spec := head_spec).
-    pure_simp; unfold head_spec; intros.
-    iIntros.
-    destruct l; Simp.
-    { iApply ewp_throw. simpl. equality. }
-    { Ret. simpl. eauto. } }
-  intros [??] (head & Hhead & -> & ->); simpl.
+    (* Struct item: [let head l = ...] *)
+    eapply structs_cons.
+    { apply struct_let_single with (spec := head_spec).
+      pure_simp; unfold head_spec; intros.
 
-  (* Struct item: [let catch_head l = ...] *)
-  eapply structs_cons.
-  { apply struct_let_single with (spec := catch_head_spec).
-    pure_simp; unfold catch_head_spec; intros.
-    iIntros. iApply ewp_call_nonrec.
-    iModIntro.
-    prove_match.
-    { (* Call to [head]. *)
-      Simp. iApply Hhead. }
-    iIntros ([h|e]).
-    { (* Value case. *)
-      iIntros "(%h0 & %t & -> & ->)".
+      (* in both cases, the expr [simp]lifies to a value or exception *)
+      destruct l.
+      - eapply pure_wp_simp; first by simp_really. apply pure_wp_throw.
+        split; eauto.
+      - pure_simp. }
+    intros [??] (head & Hhead & -> & ->); simpl.
+
+    (* Struct item: [let catch_head l = ...] *)
+    eapply structs_cons.
+    { apply struct_let_single with (spec := catch_head_spec).
+      pure_simp; unfold catch_head_spec; intros.
+      pure_enter.
+      eapply pure_eval_match'_exn.
+      - eapply pure_simp. simp. apply Hhead.
+      - intros h (t & ->). pure_simp.
+      - intros e (-> & ->). pure_simp. }
+    intros [??] (catch_head & Hcatch_head & -> & ->); simpl.
+
+    (* Struct item: [let catch_head2 l = ...] *)
+    eapply structs_cons.
+    { apply struct_let_single with (spec := catch_head_spec).
+      pure_simp; unfold catch_head_spec; intros.
+      pure_enter.
+      (* FIXME: This proof was not so pretty to begin with; but
+      we can do better here. *)
+      (* TODO: Refactor. *)
+      eapply pure_eval_match'_exn with (φ' := λ a, a = #(list.head l)) (ζ := λ e, l = [] ∧ e = VXData (Loc 0) []).
+      { eapply pure_eval_data_val; last done.
+        simpl_evals. fold eval. eapply pure_wp_Par_conseq.
+        + eapply pure_eval_app. pure_path. pure_path.
+          unfold head_spec in Hhead.
+          intros ?? <- ->. apply Hhead.
+        + eapply pure_wp_ret_singleton.
+        + intros; returns_eauto. cbn in *.
+          eapply pure_wp_ret. destruct Ha_ensures; subst.
+          red in H1; subst. encode.
+        + intros ? [ (-> & ->)| ]; cbn.
+          * eapply pure_wp_throw; eauto.
+          * Unshelve.
+            2 : { apply (λ e, l = [] ∧ e = VXData (Loc 0) []). }
+            eapply pure_wp_throw; eauto. }
+      { intros ? ->.
+        pure_match.
+        pure_path. }
+      { intros ? [-> ->]. pure_match. pure_simp. } }
+
+    intros [??] (catch_head2 & Hcatch_head2 & -> & ->); simpl.
+
+    (* We have gone though all of the struct items, time to conclude. *)
+    eapply structs_nil.
+    done.
+  Qed.
+
+End proof_pure.
+
+Section proof_effectful.
+
+  Context `{!osirisGS Σ}.
+
+  (* Calling [head #l] either returns [#h] when [l = h :: t],
+    or throws an exception when [l = []]. *)
+
+  Definition head_spec head :=
+    ∀ (A : Type) (H : Encode A) (l : list A),
+      ⊢ ewp_def top (call head #l) ⊥
+        (| RET x => ∃ h t, ⌜l = h :: t /\ x = #h⌝ ;
+        | EXN e => ⌜e = VXData (Loc 0) [] /\ l = []⌝ )%I.
+
+  (* Calling [catch_head #l] either returns [Some #h] when [l = h ::t],
+    or returns [None] when [l = []]. *)
+
+  Definition catch_head_spec catch_head :=
+    ∀ (A : Type) (H : Encode A) (l : list A),
+      ⊢ ewp_def top (call catch_head #l) ⊥
+        (RET #hopt, ⌜match l with
+                    | [] => hopt = None
+                    | h :: _ => hopt = Some h
+                    end⌝)%I.
+
+  Lemma example :
+    eval_module stdlib_with_notfound __main (λ η, True).
+  Proof.
+    unfold __main.
+    apply module_struct.
+
+    (* Struct item: [let head l = ...] *)
+    eapply structs_cons.
+    { apply struct_let_single with (spec := head_spec).
+      pure_simp; unfold head_spec; intros.
+      iIntros.
+      destruct l; Simp.
+      { iApply ewp_throw. simpl. equality. }
+      { Ret. simpl. eauto. } }
+    intros [??] (head & Hhead & -> & ->); simpl.
+
+    (* Struct item: [let catch_head l = ...] *)
+    eapply structs_cons.
+    { apply struct_let_single with (spec := catch_head_spec).
+      pure_simp; unfold catch_head_spec; intros.
+      iIntros. iApply ewp_call_nonrec.
       iModIntro.
-      next_branch.
-      next_branch.
-      { Simp. iApply ewp_value. simpl.
-        iExists (Some h0). equality. } }
-    { (* Exception case. *)
-      iIntros "[-> ->]".
-      next_branch; fold eval.
-      iApply ewp_EConstant.
-      iExists (None). done. } }
+      prove_match.
+      { (* Call to [head]. *)
+        Simp. iApply Hhead. }
+      iIntros ([h|e]).
+      { (* Value case. *)
+        iIntros "(%h0 & %t & -> & ->)".
+        iModIntro.
+        next_branch.
+        next_branch.
+        { Simp. iApply ewp_value. simpl.
+          iExists (Some h0). equality. } }
+      { (* Exception case. *)
+        iIntros "[-> ->]".
+        next_branch; fold eval.
+        iApply ewp_EConstant.
+        iExists (None). done. } }
 
-  intros [??] (catch_head & Hcatch_head & -> & ->); simpl.
+    intros [??] (catch_head & Hcatch_head & -> & ->); simpl.
 
-  (* Struct item: [let catch_head2 l = ...] *)
-  eapply structs_cons.
-  { apply struct_let_single with (spec := catch_head_spec).
-    pure_simp; unfold catch_head_spec; intros.
-    iIntros. iApply ewp_call_nonrec.
-    iModIntro.
-    prove_match.
-    { Simp. iApply ewp_bind_exn.
-      iApply ewp_mono. { iApply Hhead. }
-      iIntros ([ v | ex ]) "Houtcome".
-      - simpl.
-        iApply (ewp_value _ _ (| RET v => bi_pure(_ v); | EXN e => bi_pure(_ e))%I).
-        iDestruct "Houtcome" as "(%h & %t & -> & ->)".
-        iPureIntro.
-        instantiate (1 := (λ v, ∃ h t, l = h :: t ∧ v = (#(Some h)))).
-        simpl. eexists; eauto.
-      - simpl.
-        iDestruct "Houtcome" as "(%Hex & %Hl)".
-        iPureIntro.
-        instantiate (1 := (λ e, e = VXData {| address := 0 |} [] ∧ l = [])).
-        simpl; eauto. }
-
-    iIntros ([h|e]).
-    { (* Value case. *)
-      iIntros "(%h0 & %t & -> & ->)".
+    (* Struct item: [let catch_head2 l = ...] *)
+    eapply structs_cons.
+    { apply struct_let_single with (spec := catch_head_spec).
+      pure_simp; unfold catch_head_spec; intros.
+      iIntros. iApply ewp_call_nonrec.
       iModIntro.
-      next_branch.
-      iApply ewp_EPath. iApply ewp_value. iPureIntro. eauto. }
-    { (* Exception case. *)
-      iIntros "[-> ->]".
-      next_branch. next_branch.
-      iApply ewp_EConstant.
-      iExists (None). done. } }
+      prove_match.
+      { Simp. iApply ewp_bind_exn.
+        iApply ewp_mono. { iApply Hhead. }
+        iIntros ([ v | ex ]) "Houtcome".
+        - simpl.
+          iApply (ewp_value _ _ (| RET v => bi_pure(_ v); | EXN e => bi_pure(_ e))%I).
+          iDestruct "Houtcome" as "(%h & %t & -> & ->)".
+          iPureIntro.
+          instantiate (1 := (λ v, ∃ h t, l = h :: t ∧ v = (#(Some h)))).
+          simpl. eexists; eauto.
+        - simpl.
+          iDestruct "Houtcome" as "(%Hex & %Hl)".
+          iPureIntro.
+          instantiate (1 := (λ e, e = VXData {| address := 0 |} [] ∧ l = [])).
+          simpl; eauto. }
 
-  intros [??] (catch_head2 & Hcatch_head2 & -> & ->); simpl.
+      iIntros ([h|e]).
+      { (* Value case. *)
+        iIntros "(%h0 & %t & -> & ->)".
+        iModIntro.
+        next_branch.
+        iApply ewp_EPath. iApply ewp_value. iPureIntro. eauto. }
+      { (* Exception case. *)
+        iIntros "[-> ->]".
+        next_branch. next_branch.
+        iApply ewp_EConstant.
+        iExists (None). done. } }
 
-  (* We have gone though all of the struct items, time to conclude. *)
-  eapply structs_nil.
-  done.
-Qed.
+    intros [??] (catch_head2 & Hcatch_head2 & -> & ->); simpl.
 
-End proof.
+    (* We have gone though all of the struct items, time to conclude. *)
+    eapply structs_nil.
+    done.
+  Qed.
+
+End proof_effectful.
+
